Transform [can_wp_step] into the more subtle [not_stuck].

coq-osiris/theories/program_logic/wp_step.v
@@ -23,7 +23,7 @@ Inductive wp_step {A X} : th_config A X -> th_config_step A X -> Prop :=
     π !! ι' = None ->
     wp_step
       (σ, π, (Stop CFork (v1, v2) k), ι)
-      (σ, <[ ι' := Alive ]> π, continue k (VThread ι), [ (ι', try2 (call v1 v2) die)])
+      (σ, <[ ι' := Alive ]> π, continue k (VThread ι'), [ (ι', try2 (call v1 v2) die)])
 | JoinS :
   ∀ σ π ι k o ι',
     π !! ι' = Some (Dead o) ->
@@ -37,20 +37,41 @@ Inductive wp_step {A X} : th_config A X -> th_config_step A X -> Prop :=
       (σ, π, continue k (VThread ι), [])
 .
 
-Definition can_wp_step {A E} (c : th_config A E) := ∃ c', wp_step c c'.
+Ltac destruct_wp_step :=
+  (* For some reason, [dependent destruction] does not like it when
+     the argument [x] of [Stop] is not a variable. *)
+  try match goal with h: wp_step (?σ, ?π, Stop ?c ?x ?k, ?ι) ?m' |- _ =>
+                        remember x
+    end;
+  match goal with h: wp_step ?m ?m' |- _ =>
+                    dependent destruction h
+  end;
+  try destruct_step
+.
 
-Lemma can_step_wp_step {A E} σ (m : micro A E) :
+(* -------------------------------------------------------------------------- *)
+
+Definition not_stuck {A E} (c : th_config A E) :=
+  match c with
+  | (_, π, Stop CJoin ι' k, _) => ι' ∈ dom π
+  | (_, _, Stop CDie o _, _) => True
+  | _ => ∃ c', wp_step c c'
+  end.
+
+Lemma can_step_not_stuck {A E} σ (m : micro A E) :
   ∀ π ι,
     can_step (σ, m) ->
-    can_wp_step (σ, π, m, ι).
+    not_stuck (σ, π, m, ι).
 Proof.
   intros π ι ([σ' m'] & Hstep).
-  exists (σ', π, m', []).
-  by apply BaseS.
+  destruct_step;
+  eexists (_, π, _, []);
+    by (apply BaseS; eauto with step can_step).
+  Unshelve. apply b.
 Qed.
 
-Lemma can_wp_step_fork {A E} σ π x (k : _ -> micro A E) ι :
-  can_wp_step (σ, π, (Stop CFork x k), ι).
+Lemma not_stuck_fork {A E} σ π x (k : _ -> micro A E) ι :
+  not_stuck (σ, π, (Stop CFork x k), ι).
 Proof.
   destruct x.
   assert (exists ι', π !! ι' = None) as [ι' Hι'].
@@ -61,22 +82,22 @@ Proof.
   apply Hι'.
 Qed.
 
-Lemma can_wp_step_join {A E} σ π ι' (k : _ -> micro A E) ι o :
-  π !! ι' = Some (Dead o) ->
-  can_wp_step (σ, π, (Stop CJoin ι' k), ι).
+Lemma not_stuck_join {A E} σ π ι' (k : _ -> micro A E) ι o :
+  π !! ι' = Some o ->
+  not_stuck (σ, π, (Stop CJoin ι' k), ι).
 Proof.
-  intros.
-  eexists. apply JoinS.
-  eassumption.
+  intros Hπ; simpl.
+  apply elem_of_dom.
+  exists o; assumption.
 Qed.
 
-Lemma can_wp_step_self {A E} σ π u (k : _ -> micro A E) ι :
-  can_wp_step (σ, π, (Stop CSelf u k), ι) .
+Lemma not_stuck_self {A E} σ π u (k : _ -> micro A E) ι :
+  not_stuck (σ, π, (Stop CSelf u k), ι) .
 Proof.
   eexists. apply SelfS.
 Qed.
 
-Global Hint Resolve can_wp_step_join can_wp_step_fork can_wp_step_self : can_wp_step.
+Global Hint Resolve not_stuck_join not_stuck_fork not_stuck_self : not_stuck.
 
 Lemma invert_wp_step_resume {A E : Type} (σ σ' : store) π π' ι μ (l : loc) (o : outcome2 val exn)
   (k : outcome2 val exn → micro A E)
@@ -85,19 +106,9 @@ Lemma invert_wp_step_resume {A E : Type} (σ σ' : store) π π' ι μ (l : loc)
   wp_step (σ, π, Stop CResume (l, o) k, ι) (σ', π', m', μ) →
   σ' = <[l:=Shot]> σ ∧ m' = try2 (sk o) k ∧ π' = π ∧ μ = [].
 Proof.
-  intros.
-  dependent destruction H0.
-  pose proof (invert_step_resume _ _ _ _ _ _ _ H H0) as [??].
+  intros Hlookup Hstep.
+  destruct_wp_step.
   repeat split; auto.
+  by unfold step_resume_1; rewrite Hlookup.
+  by unfold step_resume_2; rewrite Hlookup.
 Qed.
-
-Ltac destruct_wp_step :=
-  (* For some reason, [dependent destruction] does not like it when
-     the argument [x] of [Stop] is not a variable. *)
-  try match goal with h: wp_step (?σ, ?π, Stop ?c ?x ?k, ?ι) ?m' |- _ =>
-                        remember x
-    end;
-  match goal with h: wp_step ?m ?m' |- _ =>
-                    dependent destruction h
-  end;
-  try destruct_step.
